src/HOL/IMP/Abs_Int2_ivl.thy
@@ -361,8 +361,8 @@ interpretation Abs_Int_inv
 where \<gamma> = \<gamma>_ivl and num' = num_ivl and plus' = "op +"
 and test_num' = in_ivl
 and inv_plus' = inv_plus_ivl and inv_less' = inv_less_ivl
-defines inv_aval_ivl is inv_aval''
-and inv_bval_ivl is inv_bval''
+defines inv_aval_ivl is inv_aval'
+and inv_bval_ivl is inv_bval'
 and step_ivl is step'
 and AI_ivl is AI
 and aval_ivl' is aval''
